fsFFI: model nondeterminism in read and write

basis/fsFFIScript.sml
@@ -1,4 +1,4 @@
-open preamble mlstringTheory cfHeapsBaseTheory
+open preamble mlstringTheory cfHeapsBaseTheory llistTheory
 
 val _ = new_theory"fsFFI"
 
@@ -12,24 +12,23 @@ val _ = temp_overload_on ("monad_bind", ``OPTION_BIND``)
 val _ = temp_overload_on ("monad_unitbind", ``OPTION_IGNORE_BIND``)
 (* -- *)
 
+(* infinite "streams" *)
+
+val SHD_def = Define` SHD (f : num -> num) = f 0`
+val STL_def = Define` STL (f : num -> num) = f o SUC`
+
+
 (* files: a list of file names and their content.
 *  infds: descriptor * (filename * position)
-*)
+*  numchars: stream of num modeling the nondeterministic output of read and
+*    write *)
 val _ = Datatype`
   RO_fs = <| files : (mlstring # char list) list ;
-             infds : (num # (mlstring # num)) list |>`
+             infds : (num # (mlstring # num)) list;
+             numchars : num -> num |>`
 
 val RO_fs_component_equality = theorem"RO_fs_component_equality";
 
-(* well formed file descriptor: all descriptors are < 255 
-*  and correspond to file names in files *)
-val wfFS_def = Define`
-  wfFS fs =
-    ∀fd. fd ∈ FDOM (alist_to_fmap fs.infds) ⇒
-         fd < 255 ∧
-         ∃fnm off. ALOOKUP fs.infds fd = SOME (fnm,off) ∧
-                   fnm ∈ FDOM (alist_to_fmap fs.files)
-`;
 
 (* find smallest unused descriptor index *)
 val nextFD_def = Define`
@@ -71,56 +70,77 @@ val validFD_def = Define`
   validFD fd fs ⇔ fd ∈ FDOM (alist_to_fmap fs.infds)
 `;
 
-(* increase by n the position in file descriptor *)
+(* increase by n the position in file descriptor and dump numchar's head *)
 val bumpFD_def = Define`
-  bumpFD fd fs n = fs with infds updated_by (ALIST_FUPDKEY fd (I ## ((+) n)))`
+  bumpFD fd fs n = (fs with infds updated_by (ALIST_FUPDKEY fd (I ## ((+) n))))
+                       with numchars := STL fs.numchars`
 
-(* reads (at most) n chars 
-val FDchars_def = Define`
-  FDchars fd fs n =
+(* reads several chars and update position *)
+val read_def = Define`
+  read fd fs n =
     do
       (fnm, off) <- ALOOKUP fs.infds fd ;
       content <- ALOOKUP fs.files fnm ;
-      return(TAKE (MIN (LENGTH content - off) n) content)
-    od
-`; *)
+      let k = MIN n (MIN (LENGTH content - off) (SUC (SHD fs.numchars))) in
+      return (TAKE n (DROP off content), bumpFD fd fs k)
+    od `;
 
+(* TODO: empty list implies eof *)
+(* TODO: read specification from POSIX spec. *)
+(*
+* "The value returned is the number of bytes read (zero indicates end of file)
+* and the file position is advanced by this number. It is not an error if this
+* number is smaller than the number of bytes requested; this may happen for
+* example because fewer bytes are actually available right now (maybe because we
+* were close to end-of-file, or because we are reading from a pipe, or from a
+* terminal), or because the system call was interrupted by a signal.
+*
+* Alternatively, -1 is returned when an error occurs, in such a case errno is
+* set appropriately and further it is left unspecified whether the file position
+* (if any) changes." *)
 
-(* reads several chars and update position *)
-(* axiomatic version *)
-(* TODO: valid fs? *)
-val _ = new_constant("read",``:num -> RO_fs -> num -> (string option # RO_fs)``);
-val read_spec = new_axiom("read_spec",
-``!fd fs n. 
-  case ALOOKUP fs.infds fd of
-  | NONE => (read fd fs n = (NONE, fs))
-  | SOME (fnm, off) => 
-      case ALOOKUP fs.files fnm of
-      | NONE => read fd fs n = (NONE, fs)
-      | SOME content => 
-         if off = LENGTH content then read fd fs n = (SOME [], fs)
-          else 
-            ?l. 1 <= LENGTH l /\ LENGTH l <= MIN (LENGTH content - off) n /\
-                read fd fs n = (SOME l, bumpFD fd fs (LENGTH l))``);
+val read_eof = Q.store_thm("read_eof",
+ `!fd fs n. 0 < n ⇒ (eof fd fs = SOME T) ⇒
+            read fd fs n = SOME ([], fs with numchars := STL fs.numchars)`,
+ rw[eof_def,read_def,MIN_DEF]  >>
+ qexists_tac `x` >> rw[] >>
+ cases_on `x` >> 
+ fs[DROP_LENGTH_TOO_LONG] >>
+ fs[bumpFD_def] >>
+ `ALIST_FUPDKEY fd (I ## $+ (STRLEN contents − r)) infds = infds` by 
+   (`(∀v. ALOOKUP infds fd = SOME v ⇒ (I ## $+ (STRLEN contents − r)) v = v)`
+      by (cases_on`v` >> rw[]) >>
+    imp_res_tac ALIST_FUPDKEY_unchanged) >>
+ cheat);
+
+val eof_read = Q.store_thm("eof_read",
+ `!fd fs fs' n. 0 < n ⇒ read fd fs n = SOME ([], fs) ⇒ eof fd fs = SOME T`,
+ rw[eof_def,read_def] >>
+ qexists_tac `x` >> rw[] >>
+ cases_on `x` >> 
+ fs[DROP_NIL]);
 
 (* replaces the content of the file in fs with filename fnm *)
 val write_file_def = Define`
   write_file fs fnm content = 
-    fs with files := ((fnm, content) :: (A_DELKEY fnm fs.files))`
+    (fs with files := ((fnm, content) :: (A_DELKEY fnm fs.files)))
+        with numchars := STL fs.numchars`
 
-(* writes several chars at the end of the file *)
-val _ = new_constant("write",``:num -> num -> string -> RO_fs -> (num option # RO_fs)``);
-val write_spec = new_axiom("read_spec",
-``!fd fs n chars fs. 
-  case ALOOKUP fs.infds fd of
-  | NONE => (write fd n chars fs = (NONE, fs))
-  | SOME (fnm, off) => 
-      case ALOOKUP fs.files fnm of
-      | NONE => write fd n chars fs = (NONE, fs)
-      | SOME content => (n <= LENGTH chars =>
-          (?k. k <= MIN (LENGTH content - off) n /\
-               write fd n chars fs = 
-                 (SOME k, write_file fs fnm (content ++ TAKE k chars))))``);
+(* "The write function returns the number of bytes successfully written into the
+*  array, which may at times be less than the specified nbytes. It returns -1 if
+*  an exceptional condition is encountered." *) 
+(* can it be 0? *)
+
+val write_def = Define`
+  write fd n chars fs =
+    do
+      (fnm, off) <- ALOOKUP fs.infds fd ;
+      content <- ALOOKUP fs.files fnm ;
+      assert(n <= LENGTH chars);
+      let k = MIN n (SHD fs.numchars) in
+      return (k, write_file fs fnm (content ++ TAKE k chars))
+    od `;
+
 
 (* remove file from file descriptor *)
 val closeFD_def = Define`
@@ -156,7 +176,7 @@ val getNullTermStr_def = Define`
 (* read file name from the first non null bytes
 *  open the file with read access
 *  write its file descriptor index in the first byte *)
-val ffi_open_def = Define`
+val ffi_open_in_def = Define`
   ffi_open bytes fs =
     do
       fname <- getNullTermStr bytes;
@@ -167,7 +187,7 @@ val ffi_open_def = Define`
     return (LUPDATE 255w 0 bytes, fs)`;
 
 (* open with write access to the end of file *)
-val ffi_open_append_def = Define`
+val ffi_open_out_def = Define`
   ffi_open_append bytes fs =
     do
       fname <- getNullTermStr bytes;
@@ -187,16 +207,15 @@ val ffi_read_def = Define`
     do
     (* the buffer contains at least the number of requested bytes *)
       assert(LENGTH bytes >= w2n (HD (TL bytes)) + 2);
-      let (lo, fs') = read (w2n (HD bytes)) fs (w2n (HD (TL bytes))) in
-      case lo of
-      (* return error code *)
-      | NONE => return ([1w], fs') 
+      (l, fs') <- read (w2n (HD bytes)) fs (w2n (HD (TL bytes)));
       (* return ok code and list of chars
       *  the end of the array may remain unchanged *)
-      | SOME l => return (0w :: n2w (LENGTH l) ::
-                          MAP (n2w o ORD) l ++
-                          DROP (LENGTH l +2) bytes, fs')
-      od`;
+      return (0w :: n2w (LENGTH l) ::
+              MAP (n2w o ORD) l ++
+              DROP (LENGTH l +2) bytes, fs')
+      od ++ return ([1w], fs)`;
+      (* inaccurate: "when an error occurs, [...] 
+      * it is left unspecified whether the file position (if any) changes. *)
 
 (* [descriptor index; number of chars to write; chars to write]
 *    -> [return code; number of written chars]
@@ -204,12 +223,11 @@ val ffi_read_def = Define`
 * ssize_t write(int fildes, const void *buf, size_t nbytes) *)
 val ffi_write_def = Define`
   ffi_write bytes fs =
-    let (no, fs') = write (w2n (HD bytes)) (w2n (HD (TL bytes))) 
-                          (MAP (CHR o w2n) (TL (TL bytes))) fs in
     do
     (* the buffer contains at least the number of requested bytes *)
       assert(LENGTH bytes >= 2);
-      nw <- no;  
+      (nw, fs') <- write (w2n (HD bytes)) (w2n (HD (TL bytes))) 
+                         (MAP (CHR o w2n) (TL (TL bytes))) fs;
       (* return ok code and list of chars *)
       return ([0w; n2w nw], fs')
     (* return error code *)
